Translation/Term/Lemmas.lean
@@ -497,7 +497,10 @@ case annot ih =>
 case hole =>
   sorry
 
-
+theorem Translation.synth_term_completeness :
+  Core.Translation.SynthTerm G Δ Γ T t ->
+  T.synth_term G Δ Γ = some t ∧
+  t.Determined ∧ G&Δ, Γ ⊢ t : T := by sorry
 
 
 
@@ -515,25 +518,33 @@ theorem Translation.Term.Sound2
 
   Surface.Translation.Term G G' Δ Γ t T Δ' Γ' t' T' ->
 
-  (t.type_directed_translate G' Δ' Γ' T' = some t' ∧
+  t.type_directed_translate G' Δ' Γ' T = some t' ∧
    t'.Determined ∧
-   G'&Δ',Γ' ⊢ t' : T') := by
+   G'&Δ',Γ' ⊢ t' : T' := by
 intro wf h1 wfc h2 h3 h4
 induction h4 <;> simp [Surface.Term.type_directed_translate] at *
-case var x τ Γ' T' Δ Δ' Γ j1 j2 j3 =>
-  have lem := Translation.Ty.sound2 wf j3 h1 h2
+case var x T A Γ' Δ Δ' A' T' d  Γ _ _ j1 j2 j3 =>
+  have lem := Translation.Ty.sound2 wf j1 h1 h2
   simp at *; cases lem.1; simp at lem
+  have lem' := Translation.Ty.sound2 wf j2 h1 h2
+  simp at *; cases lem'.1; simp at lem'
   apply And.intro
-  · apply j2
+  · split <;> simp at *
+    · sorry
+    · sorry
   · apply And.intro
-    apply Core.Term.Determined.var
-    apply Core.Typing.var; assumption; apply lem
+    · sorry
+    · sorry; -- apply Core.Typing.var; assumption; apply lem
 sorry
 sorry
+case appP Δ A Δ' A' Γ f B Γ' f' B' t' j1 j2 j3 ih =>
+  replace ih := ih h2 h3
+  rcases ih with ⟨ih1, ih2, ih3⟩
+
+  sorry
 sorry
 sorry
-sorry
-sorry
+case lamt => sorry
 case annot Δ Ta Δ' Ta' Tb Tb' Γ' c Γ t t' j1 j2 j3 j4 j5 =>
   replace j5 := j5 h2 h3
   rcases j5 with ⟨j5, j6⟩
@@ -543,20 +554,13 @@ case annot Δ Ta Δ' Ta' Tb Tb' Γ' c Γ t t' j1 j2 j3 j4 j5 =>
   have lem' := Translation.Ty.sound2 wf j2 h1 h2
   rcases lem' with ⟨lem1', lem2', lem3'⟩
   subst lem2'
+  have lem3 := Translation.synth_term_completeness j3
   apply And.intro
   · rw[Option.bind_eq_some_iff]; exists t';
-    apply And.intro;
-    · apply j5
-    · rw[Option.bind_eq_some_iff]; exists c;
-      apply And.intro
-      · sorry
-      · simp
   · apply And.intro
     · apply Core.Term.Determined.cast.1; apply And.intro
       · apply j6.1
-      sorry
-    · apply Core.Typing.cast;
-      · sorry
-      · sorry
-      · sorry
-      · sorry
+      · apply lem3.2.1
+    · apply Core.Typing.cast
+      · apply j6.2
+      · apply lem3.2.2
